src/Crypto/AESEncryption.dfy
@@ -8,8 +8,8 @@ module {:extern "AESEncryption"} AESEncryption {
   import opened UInt = StandardLibrary.UInt
 
   export
-    provides AESDecryptWrapper, AESEncryptWrapper, AESDecrypt, AESEncrypt, EncryptionSuites, StandardLibrary, UInt, PlaintextDecryptedWithAAD, EncryptionOutputEncryptedWithAAD
-    provides IsEncrypted
+    provides AESDecrypt, AESEncrypt, AESDecrypt, AESEncrypt, EncryptionSuites, StandardLibrary, 
+      UInt, PlaintextDecryptedWithAAD, EncryptionOutputEncryptedWithAAD, CiphertextGeneratedWithPlaintext
     reveals EncryptionOutput
 
   datatype EncryptionOutput = EncryptionOutput(cipherText: seq<uint8>, authTag: seq<uint8>)
@@ -19,7 +19,7 @@ module {:extern "AESEncryption"} AESEncryption {
   // in order to ensure that the AAD used is as expected.
   predicate {:axiom} PlaintextDecryptedWithAAD(plaintext: seq<uint8>, aad: seq<uint8>)
   predicate {:axiom} EncryptionOutputEncryptedWithAAD(ciphertext: EncryptionOutput, aad: seq<uint8>)
-  predicate {:axiom} IsEncrypted (ciphertext: seq<uint8>, plaintext: seq<uint8>)
+  predicate {:axiom} CiphertextGeneratedWithPlaintext (ciphertext: seq<uint8>, plaintext: seq<uint8>)
 
   function method EncryptionOutputFromByteSeq(s: seq<uint8>, encAlg: EncryptionSuites.EncryptionSuite): (encArt: EncryptionOutput)
     requires encAlg.Valid()
@@ -30,7 +30,7 @@ module {:extern "AESEncryption"} AESEncryption {
     EncryptionOutput(s[.. |s| - encAlg.tagLen as int], s[|s| - encAlg.tagLen as int ..])
   }
 
-  method {:extern "AESEncryption.AES_GCM", "AESEncrypt"} AESEncrypt(encAlg: EncryptionSuites.EncryptionSuite, iv: seq<uint8>, key: seq<uint8>, msg: seq<uint8>, aad: seq<uint8>)
+  method {:extern "AESEncryption.AES_GCM", "AESEncryptExtern"} AESEncryptExtern(encAlg: EncryptionSuites.EncryptionSuite, iv: seq<uint8>, key: seq<uint8>, msg: seq<uint8>, aad: seq<uint8>)
       returns (res : Result<EncryptionOutput>)
     requires encAlg.Valid()
     requires encAlg.alg.AES?
@@ -38,9 +38,9 @@ module {:extern "AESEncryption"} AESEncryption {
     requires |iv| == encAlg.ivLen as int
     requires |key| == encAlg.keyLen as int
     ensures res.Success? ==> EncryptionOutputEncryptedWithAAD(res.value, aad)
-    ensures res.Success? ==> IsEncrypted(res.value.cipherText, msg)
+    ensures res.Success? ==> CiphertextGeneratedWithPlaintext(res.value.cipherText, msg)
 
-  method AESEncryptWrapper(encAlg: EncryptionSuites.EncryptionSuite, iv: seq<uint8>, key: seq<uint8>, msg: seq<uint8>, aad: seq<uint8>)
+  method AESEncrypt(encAlg: EncryptionSuites.EncryptionSuite, iv: seq<uint8>, key: seq<uint8>, msg: seq<uint8>, aad: seq<uint8>)
       returns (res : Result<EncryptionOutput>)
     requires encAlg.Valid()
     requires encAlg.alg.AES?
@@ -50,14 +50,14 @@ module {:extern "AESEncryption"} AESEncryption {
     ensures res.Success? ==>
       |res.value.cipherText| == |msg| && |res.value.authTag| == encAlg.tagLen as int
     ensures res.Success? ==> EncryptionOutputEncryptedWithAAD(res.value, aad)
-    ensures res.Success? ==> IsEncrypted(res.value.cipherText, msg)
+    ensures res.Success? ==> CiphertextGeneratedWithPlaintext(res.value.cipherText, msg)
     {
-      res := AESEncrypt(encAlg, iv, key, msg, aad);
+      res := AESEncryptExtern(encAlg, iv, key, msg, aad);
       expect res.Success? ==> |res.value.cipherText| == |msg|;
       expect res.Success? ==> |res.value.authTag| == encAlg.tagLen as int;
     }
 
-  method {:extern "AESEncryption.AES_GCM", "AESDecrypt"} AESDecrypt(encAlg: EncryptionSuites.EncryptionSuite, key: seq<uint8>, cipherTxt: seq<uint8>, authTag: seq<uint8>, iv: seq<uint8>, aad: seq<uint8>)
+  method {:extern "AESEncryption.AES_GCM", "AESDecryptExtern"} AESDecryptExtern(encAlg: EncryptionSuites.EncryptionSuite, key: seq<uint8>, cipherTxt: seq<uint8>, authTag: seq<uint8>, iv: seq<uint8>, aad: seq<uint8>)
       returns (res: Result<seq<uint8>>)
     requires encAlg.Valid()
     requires encAlg.alg.AES?
@@ -66,9 +66,9 @@ module {:extern "AESEncryption"} AESEncryption {
     requires |iv| == encAlg.ivLen as int
     requires |authTag| == encAlg.tagLen as int
     ensures res.Success? ==> PlaintextDecryptedWithAAD(res.value, aad)
-    ensures res.Success? ==> IsEncrypted(cipherTxt, res.value) 
+    ensures res.Success? ==> CiphertextGeneratedWithPlaintext(cipherTxt, res.value) 
 
-  method AESDecryptWrapper(encAlg: EncryptionSuites.EncryptionSuite, key: seq<uint8>, cipherTxt: seq<uint8>, authTag: seq<uint8>, iv: seq<uint8>, aad: seq<uint8>)
+  method AESDecrypt(encAlg: EncryptionSuites.EncryptionSuite, key: seq<uint8>, cipherTxt: seq<uint8>, authTag: seq<uint8>, iv: seq<uint8>, aad: seq<uint8>)
       returns (res: Result<seq<uint8>>)
     requires encAlg.Valid()
     requires encAlg.alg.AES?
@@ -78,9 +78,9 @@ module {:extern "AESEncryption"} AESEncryption {
     requires |authTag| == encAlg.tagLen as int
     ensures res.Success? ==> |res.value| == |cipherTxt|
     ensures res.Success? ==> PlaintextDecryptedWithAAD(res.value, aad)
-    ensures res.Success? ==> IsEncrypted(cipherTxt, res.value)
+    ensures res.Success? ==> CiphertextGeneratedWithPlaintext(cipherTxt, res.value)
     {
-      res := AESDecrypt(encAlg, key, cipherTxt, authTag, iv, aad);
+      res := AESDecryptExtern(encAlg, key, cipherTxt, authTag, iv, aad);
       expect res.Success? ==> |cipherTxt| == |res.value|;
     }
 
